wip: fix hash & address proofs

proof/correctness/Correctness_Hash.ec
@@ -3,324 +3,423 @@ pragma Goals : printall.
 require import AllCore List RealExp IntDiv.
 from Jasmin require import JModel.
 
-require import XMSS_IMPL.
-require import Types Address Notation Hash Primitives Params Parameters Utils Util.
-require import Correctness_Mem.
+require import XMSS_IMPL Parameters.
+require import Params Address Hash.
+require import Correctness_Mem Correctness_Address.
 
 require import Array8 Array32 Array64 Array96 Array128.
 
-
 axiom hash_96 (x : W8.t Array96.t) :
-    phoare[M(Syscall).__core_hash_96 : arg.`2 = x ==> to_list res = Hash (to_list x)] = 1%r.
+  phoare[
+      M(Syscall).__core_hash_96 : 
+      arg.`2 = x 
+      ==>  
+      to_list res = val (Hash (to_list x))
+    ] = 1%r.
 
 axiom hash_128 (x : W8.t Array128.t) :
-    phoare[M(Syscall).__core_hash_128 : arg.`2 = x ==> to_list res = Hash (to_list x)] = 1%r.
+  phoare[
+      M(Syscall).__core_hash_128 : 
+      arg.`2 = x 
+      ==> 
+      to_list res = val (Hash (to_list x))
+    ] = 1%r.
 
 lemma prf_correctness (a b : W8.t Array32.t) :
+    n = XMSS_N /\
     prf_padding_val = XMSS_HASH_PADDING_PRF /\ 
     padding_len = XMSS_PADDING_LEN =>
     equiv [
     M(Syscall).__prf ~ Hash.prf : 
-    arg{1}.`2 = a /\ arg{1}.`3 = b /\ arg{2} = (to_list a, to_list b) 
+    arg{1}.`2 = a /\ 
+    arg{1}.`3 = b /\ 
+    arg{2} = (to_list a, NBytes.insubd (to_list b)) 
     ==>
-    res{2} = to_list res{1}
+    val res{2} = to_list res{1}
     ].
 proof.
-rewrite /XMSS_HASH_PADDING_PRF /XMSS_PADDING_LEN => [#] ??.
+rewrite /XMSS_N /XMSS_HASH_PADDING_PRF /XMSS_PADDING_LEN => [#] n_val ??.
 proc.
 seq 9 2 : (buf{2} = to_list buf{1}); last first.
   + inline M(Syscall).__core_hash__96 M(Syscall)._core_hash_96; wp; sp.
     ecall {1} (hash_96 buf{1}); auto => /> /#.
 seq 3 0 : (#pre); 1:auto.
 seq 1 1 : (#pre /\ padding{2} = to_list padding_buf{1}).
-  + call {1} (ull_to_bytes_correct (of_int 3)%W64); auto => />. 
+  + admit.
+    (* FIXME: Used to be call {1} (ull_to_bytes_correct (of_int 3)%W64); auto => />. *) 
 seq 1 0 : (
-  key{2} = to_list key{1} /\
+  val key{2} = to_list key{1} /\
   in_0{2} = to_list in_0{1} /\
   padding{2} = to_list padding_buf{1} /\ 
   forall (k : int), 0 <= k < 32 => buf{1}.[k] = nth witness padding{2} k
-); first by auto => /> *; smt(@Array96 @List).
+).
+    + auto => /> &1; split.  
+         - rewrite insubdK /P //= size_to_list n_val //.  
+         - move => k??.
+           rewrite initiE 1:/# => />.  
+           by rewrite ifT. 
+
 seq 1 0 : (#pre /\ aux{1} = key{1}); first by ecall {1} (_x_memcpy_u8u8_post key{1}); auto => />.
-seq 1 0 : (#pre /\ forall (k : int), 32 <= k < 64 => buf{1}.[k] = nth witness key{2} (k - 32)).
-    + auto => />; smt(@Array96 @List).
+seq 1 0 : (#pre /\ forall (k : int), 32 <= k < 64 => buf{1}.[k] = nth witness (val key{2}) (k - 32)).
+    + auto => /> &1 &2 H0 H1; split => k??.  
+         - rewrite initiE 1:/# => />.     
+           rewrite ifF 1:/#. 
+           apply H1 => //. 
+         - rewrite initiE 1:/# => />. 
+           rewrite ifT //= H0 get_to_list //=.
 seq 1 0 : (
-  key{2} = to_list key{1} /\
+  val key{2} = to_list key{1} /\
   in_0{2} = to_list in_0{1} /\
   padding{2} = to_list padding_buf{1} /\ 
   (forall (k : int), 0 <= k < 32 => buf{1}.[k] = nth witness padding{2} k) /\
-  (forall (k : int), 32 <= k < 64 => buf{1}.[k] = nth witness key{2} (k - 32)) /\
+  (forall (k : int), 32 <= k < 64 => buf{1}.[k] = nth witness (val key{2}) (k - 32)) /\
   aux{1} = in_0{1}
 ).
     + ecall {1} (_x_memcpy_u8u8_post in_0{1}); auto => /> /#.
 seq 1 0 : (
-  key{2} = to_list key{1} /\ size key{2} = 32 /\
-  in_0{2} = to_list in_0{1} /\ size in_0{2} = 32 /\
-  padding{2} = to_list padding_buf{1} /\  size padding{2} = 32 /\
+  val key{2} = to_list key{1} /\
+  in_0{2} = to_list in_0{1} /\ 
+  size in_0{2} = 32 /\
+  padding{2} = to_list padding_buf{1} /\ 
+  size padding{2} = 32 /\
   (forall (k : int), 0 <= k < 32 => buf{1}.[k] = nth witness padding{2} k) /\
-  (forall (k : int), 32 <= k < 64 => buf{1}.[k] = nth witness key{2} (k - 32)) /\
+  (forall (k : int), 32 <= k < 64 => buf{1}.[k] = nth witness (val key{2}) (k - 32)) /\
   (forall (k : int), 64 <= k < 96 => buf{1}.[k] = nth witness in_0{2} (k - 64))
 ).
-    + auto => /> *; do split; smt(@Array96 @List).
-    + auto => /> *; rewrite !/to_list !/mkseq -!iotaredE => /> /#. 
+    + auto => /> &1 &2 H0 H1 H2.
+      do split; 1,2: by rewrite size_to_list. 
+         - move => k??. 
+           rewrite initiE 1:/# => />.
+           rewrite ifF 1:/#. 
+           apply H1 => //. 
+         - move => k??. 
+           rewrite initiE 1:/# => />.
+           rewrite ifF 1:/#. 
+           apply H2 => //. 
+         - move => k??. 
+           rewrite initiE 1:/# => />.
+           by rewrite ifT.          
+auto => /> &1 &2 H0 H1 H2 H3 H4 H5. 
+apply (eq_from_nth witness); [ by rewrite !size_cat H0 !size_to_list |].
+rewrite !size_cat H0 !size_to_list //= => i?. 
+case (0 <= i < 32).
+    + move => ?.
+      rewrite nth_cat size_cat !size_to_list ifT 1:/# nth_cat !size_to_list ifT 1:/# get_to_list /#. 
+case (32 <= i < 64).
+    + move => ?_.
+      rewrite nth_cat size_cat !size_to_list ifT 1:/# nth_cat size_to_list ifF 1:/# -H0 /#. 
+(* At this point, we know that 64 <= k < 96 *)
+move => ??.
+rewrite nth_cat size_cat !size_to_list ifF 1:/# get_to_list /#. 
 qed.
 
 lemma prf_keygen_correctness (a : W8.t Array64.t, b : W8.t Array32.t) :
+    n = XMSS_N /\
     prf_padding_val = XMSS_HASH_PADDING_PRF /\
     prf_kg_padding_val = XMSS_HASH_PADDING_PRF_KEYGEN /\ 
     padding_len = XMSS_PADDING_LEN =>
     equiv [
-    M(Syscall).__prf_keygen ~ Hash.prf_keygen : 
-    arg{1}.`2 = a /\ arg{1}.`3 = b /\ arg{2} = (to_list a, to_list b) 
-    ==>
-    res{2} = to_list res{1}
+      M(Syscall).__prf_keygen ~ Hash.prf_keygen : 
+      arg{1}.`2 = a /\ 
+      arg{1}.`3 = b /\ 
+      arg{2} = (to_list a, NBytes.insubd (to_list b))
+      ==>
+      val res{2} = to_list res{1}
     ].
 proof.
-rewrite /XMSS_HASH_PADDING_PRF_KEYGEN /XMSS_PADDING_LEN => [#] ???.
+rewrite /XMSS_N /XMSS_HASH_PADDING_PRF_KEYGEN /XMSS_PADDING_LEN.
+move => [#] n_val ???.
 proc => //=.
 seq 9 2 : (buf{2} = to_list buf{1}); last first.
   + inline M(Syscall).__core_hash__128 M(Syscall)._core_hash_128; wp; sp.
     ecall {1} (hash_128 buf{1}); auto => /> /#.
 seq 3 0 : (#pre); 1:auto.
 seq 1 1 : (#pre /\ padding{2} = to_list padding_buf{1}).
-  + call {1} (ull_to_bytes_correct (of_int 4)%W64); auto => />. 
+  + admit. (* call {1} (ull_to_bytes_correct (of_int 4)%W64); auto => />.*)
 seq 1 0 : (
-  key{2} = to_list key{1} /\
+  val key{2} = to_list key{1} /\
   in_0{2} = to_list in_0{1} /\
   padding{2} = to_list padding_buf{1} /\ 
   forall (k : int), 0 <= k < 32 => buf{1}.[k] = nth witness padding{2} k
-); first by auto => /> *; smt(@Array128 @List).
+).
+    + auto => /> &1; split.
+         * rewrite NBytes.insubdK // /P size_to_list n_val //.
+         * move => k??.
+           rewrite initiE 1:/# => />. 
+           by rewrite ifT.
 seq 1 0 : (#pre /\ aux{1} = key{1}); first by ecall {1} (_x_memcpy_u8u8_post key{1}); auto => />.
-seq 1 0 : (#pre /\ forall (k : int), 32 <= k < 64 => buf{1}.[k] = nth witness key{2} (k - 32)).
-    + auto => />; smt(@Array128 @List).
 seq 1 0 : (
-  key{2} = to_list key{1} /\
+    #pre /\ 
+    forall (k : int), 32 <= k < 64 => buf{1}.[k] = nth witness (val key{2}) (k - 32)
+).
+    + auto => /> &1 &2 H0 H1; split => k??.
+         * rewrite initiE 1:/# => />. 
+           rewrite ifF 1:/#.
+           apply H1 => //.
+         * rewrite initiE 1:/# => />.
+           by rewrite ifT 1:/# H0 get_to_list.           
+seq 1 0 : (
+  val key{2} = to_list key{1} /\
   in_0{2} = to_list in_0{1} /\
   padding{2} = to_list padding_buf{1} /\ 
   (forall (k : int), 0 <= k < 32 => buf{1}.[k] = nth witness padding{2} k) /\
-  (forall (k : int), 32 <= k < 64 => buf{1}.[k] = nth witness key{2} (k - 32)) /\
+  (forall (k : int), 32 <= k < 64 => buf{1}.[k] = nth witness (val key{2}) (k - 32)) /\
   aux_0{1} = in_0{1}
 ).
     + ecall {1} (_x_memcpy_u8u8_64_post in_0{1}); auto => /> /#.
 seq 1 0 : (
-  key{2} = to_list key{1} /\ size key{2} = 32 /\
-  in_0{2} = to_list in_0{1} /\ size in_0{2} = 64 /\
-  padding{2} = to_list padding_buf{1} /\  size padding{2} = 32 /\
+  val key{2} = to_list key{1} /\
+  in_0{2} = to_list in_0{1} /\ 
+  size in_0{2} = 64 /\
+  padding{2} = to_list padding_buf{1} /\
   (forall (k : int), 0 <= k < 32 => buf{1}.[k] = nth witness padding{2} k) /\
-  (forall (k : int), 32 <= k < 64 => buf{1}.[k] = nth witness key{2} (k - 32)) /\
+  (forall (k : int), 32 <= k < 64 => buf{1}.[k] = nth witness (val key{2}) (k - 32)) /\
   (forall (k : int), 64 <= k < 128 => buf{1}.[k] = nth witness in_0{2} (k - 64))
 ).
-    + auto => /> *; do split; smt(@Array128 @List).
-    + auto => /> *; rewrite !/to_list !/mkseq -!iotaredE => /> /#. 
+    + auto => /> &1 &2 H0 H1 H2; do split. 
+         * by rewrite size_to_list.  
+         * move => k??.
+           rewrite initiE 1:/# => />.
+           rewrite ifF 1:/#.
+           apply H1 => //.
+         * move => k??.
+           rewrite initiE 1:/# => />.
+           rewrite ifF 1:/#. 
+           apply H2 => //.
+         * move => k??.
+           rewrite initiE 1:/# => />.
+           by rewrite ifT 1:/#. 
+auto => /> &1 &2 H0 H1 H2 H3 H4.
+apply (eq_from_nth witness). 
+    + rewrite !size_cat H0 !size_to_list //=.
+rewrite !size_cat H0 !size_to_list => i?.
+case (0 <= i < 32).
+    + move => ?.
+      rewrite nth_cat !size_cat !size_to_list //= ifT 1:/#.
+      rewrite nth_cat !size_to_list //= ifT /#.
+case (32 <= i < 64). 
+    + move => ?_.
+      rewrite nth_cat !size_cat !size_to_list //= ifT 1:/#.
+      rewrite nth_cat !size_to_list //= ifF 1:/#.
+      rewrite -!get_to_list -H0 /#.
+move => ??.
+rewrite nth_cat !size_cat !size_to_list //= ifF /#.
 qed.
 
+op merge_nbytes_to_array (a b : nbytes) : W8.t Array64.t = 
+  Array64.init (fun i => if 0 <= i < 32 
+                         then nth witness (val a) i 
+                         else nth witness (val b) (i - 32)).
 
- 
 lemma rand_hash_correct (i0 i1: nbytes, _pub_seed : W8.t Array32.t, _in : W8.t Array64.t, a : W32.t Array8.t) :
     padding_len = XMSS_PADDING_LEN /\ 
     prf_padding_val = XMSS_HASH_PADDING_PRF /\
     padding_len = XMSS_PADDING_LEN /\ 
-    n = XMSS_N /\
-    size i0 = n /\ 
-    size i1 = n =>
+    n = XMSS_N  =>
     equiv [
       M(Syscall).__thash_h ~ Hash.rand_hash :
       arg{1}.`2 = (merge_nbytes_to_array i0 i1) /\
       arg{1}.`3 = _pub_seed /\
       arg{1}.`4 = a /\
-      arg{2} = (i0, i1, to_list _pub_seed, a)
+      arg{2} = (i0, i1, NBytes.insubd(to_list _pub_seed), a)
       ==>
-      to_list res{1}.`1 = res{2}.`1 /\
+      to_list res{1}.`1 = val res{2}.`1 /\
       res{1}.`2 = res{2}.`2
     ].
 proof.
 rewrite /XMSS_PADDING_LEN /XMSS_HASH_PADDING_PRF /XMSS_PADDING_LEN /XMSS_N => [#] ??? nval.
-rewrite nval => ??.
 proc; auto => />.
 seq 3 0 : (#pre); 1:auto.
 seq 1 1 : (#pre /\ padding{2} = to_list aux{1} /\ size padding{2} = 32).
-    + by call {1} (ull_to_bytes_correct W64.one); skip => /> &1 &2 *; rewrite size_to_list.
+    + admit. 
+(* by call {1} (ull_to_bytes_correct W64.one); skip => /> &1 &2 *; rewrite size_to_list. *)
 swap {1} [2..3] -1.
 
 (* conseq to rewrite #pre *)
 conseq (: 
-  to_list in_0{1} = _left{2} ++ _right{2} /\
-  _seed{2} = to_list pub_seed{1} /\ 
+  to_list in_0{1} = (val _left{2}) ++ (val _right{2}) /\
+  val _seed{2} = to_list pub_seed{1} /\ 
   address{2} = addr{1} /\
-  padding{2} = to_list aux{1} /\ 
-  
-  size _left{2} = 32 /\
-  size _right{2} = 32 /\
+  padding{2} = to_list aux{1} /\   
   size padding{2} = 32
-
   ==> 
   _
 ).
-auto => /> &1 *. rewrite /merge_nbytes_to_array. apply (eq_from_nth witness); [ rewrite size_cat size_to_list /# | smt(@List @Array64) ]. 
-(* ; first by auto => /> &1 ?; split; move => k Hk1 Hk2; rewrite /merge_nbytes_to_array initE; auto => />; rewrite ifT 1:/#; auto => /> /#. => se usar forall em vez de in=left++right*) 
+    + auto => /> &1 ?; split. 
+         * apply (eq_from_nth witness). 
+print NBytes.valP.
+             - by rewrite size_to_list size_cat (: size (val i0) = 32) 1:#smt:(NBytes.valP) (: size (val i1) = 32) 1:#smt:(NBytes.valP).
+           rewrite size_to_list => j?. 
+           rewrite get_to_list /merge_nbytes_to_array initiE 1:/# => />. 
+           case (0 <= j < 32) => ?. 
+             - by rewrite nth_cat (: size (val i0) = 32) 1:#smt:(NBytes.valP) ifT 1:/#.
+           by rewrite nth_cat (: size (val i0) = 32) 1:#smt:(NBytes.valP) ifF 1:/#. 
+         * by rewrite NBytes.insubdK //= /P size_to_list nval.
 seq 2 2 : (#pre /\ addr_bytes{2} = to_list addr_as_bytes{1}).
     + inline {1} M(Syscall).__set_key_and_mask; ecall {1} (addr_to_bytes_correctness addr{1}); auto => /> /#. 
 seq 1 0 : (
   #pre /\
   forall (k : int), 0 <= k < 32 => buf{1}.[k] = nth witness padding{2} k
 ); first by auto => /> *; rewrite initE ifT 1:/#; auto => /> /#.
- 
 seq 1 1 : (
-  to_list in_0{1} = _left{2} ++ _right{2} /\
+  to_list in_0{1} = (val _left{2}) ++ (val _right{2}) /\
   
-  _seed{2} = to_list pub_seed{1} /\ 
+  val _seed{2} = to_list pub_seed{1} /\ 
   address{2} = addr{1} /\
   addr_bytes{2} = to_list addr_as_bytes{1} /\
-
-  size _left{2} = n /\
-  size _right{2} = n /\
   size padding{2} = 32 /\
-  size key{2} = 32 /\
 
-  (* Tmp *)
-  key{2} = to_list aux{1} /\
-
-  (* Towards #post *)
+  val key{2} = to_list aux{1} /\
   forall (k : int), 0 <= k < 32 => buf{1}.[k] = nth witness padding{2} k
 ).
     + inline {1} M(Syscall).__prf_ M(Syscall)._prf; wp; sp.
-      exists * in_01{1}, key0{1}; elim * => _P1 _P2; call {1} (prf_correctness _P1 _P2); first by split; assumption. 
-      skip => /> &1 &2 *. rewrite size_to_list; do split; 1,2: rewrite nval; assumption.
+      exists * in_01{1}, key0{1}; elim * => _P1 _P2; call {1} (prf_correctness _P1 _P2); first by smt(). 
+      skip => /> &1 &2 ? H0 *.
+      rewrite -H0 #smt:(@NBytes).
 (* Remove hash from #post *)
 seq 11 6 : (
   addr{1} = address{2} /\
-  to_list buf{1} = padding{2} ++ key{2} ++ nbytexor (_left{2} ++ _right{2}) (bitmask_0{2} ++ bitmask_1{2})
+  to_list buf{1} = padding{2} ++ (val key{2}) ++ bytexor ((val _left{2}) ++ (val _right{2})) ((val bitmask_0{2}) ++ (val bitmask_1{2}))
 ); last first. 
-    + inline {1}  M(Syscall)._core_hash_128. wp. ecall {1} (hash_128 in_00{1}). auto => /> &1 &2 ??; move => ->; congr.      
+    + inline {1}  M(Syscall)._core_hash_128. 
+      wp. 
+      ecall {1} (hash_128 in_00{1}). 
+      auto => /> &1 &2 ?_ ->.
+      by do congr. 
 seq 1 0 : (
     #pre /\
-    forall (k : int), 0 <= k < 32 => buf{1}.[32 + k] = nth witness key{2} k
+    forall (k : int), 0 <= k < 32 => buf{1}.[32 + k] = nth witness (val key{2}) k
 ).
-    + auto => /> &1 &2 *; split; move => ???; rewrite initE ifT 1:/#; auto => />; [rewrite ifF /# | rewrite ifT /#].
+    + auto => /> &1 &2 ??? H *; split => k??; rewrite initiE 1:/# => />.
+         * rewrite ifF /#.                       
+         * by rewrite ifT 1:/# H get_to_list.
 seq 2 2 : (#pre).
     + inline {1} M(Syscall).__set_key_and_mask; ecall {1} (addr_to_bytes_correctness addr{1}); auto => /> /#.
-(* Bitmask appears first here *)
 seq 2 1 : (
-  to_list in_0{1} = _left{2} ++ _right{2} /\
-  _seed{2} = to_list pub_seed{1} /\ 
+  to_list in_0{1} = val _left{2} ++ val _right{2} /\
+  val _seed{2} = to_list pub_seed{1} /\ 
   address{2} = addr{1} /\
   addr_bytes{2} = to_list addr_as_bytes{1} /\
 
-  size _left{2} = n /\
-  size _right{2} = n /\
   size padding{2} = 32 /\
-  size key{2} = 32 /\
-  
-  (* Bitmask *)
-  (forall (k : int), 0 <= k < 32 => bitmask{1}.[k] = nth witness bitmask_0{2} k) /\
-  size bitmask_0{2} = n /\
+    
+  (forall (k : int), 0 <= k < 32 => bitmask{1}.[k] = nth witness (val bitmask_0{2}) k) /\
 
-  (* Towards #post *)
   (forall (k : int), 0 <= k < 32 => buf{1}.[k] = nth witness padding{2} k) /\
-  (forall (k : int), 0 <= k < 32 => buf{1}.[32 + k] = nth witness key{2} k)
+  (forall (k : int), 0 <= k < 32 => buf{1}.[32 + k] = nth witness (val key{2}) k)
 ).
     + inline {1} M(Syscall).__prf_ M(Syscall)._prf; wp; sp.
-      exists * in_01{1}, key0{1}; elim * => _P1 _P2; call {1} (prf_correctness _P1 _P2); first by split; assumption.
-      skip => /> &1 &2 *. split; [| rewrite size_to_list /# ]. move => k Hk0 Hk1. rewrite initiE 1:/#.
-      auto => />. rewrite ifT; split; [| move => _]; assumption.
+      exists * in_01{1}, key0{1}; elim * => _P1 _P2; call {1} (prf_correctness _P1 _P2); first by smt().
+      skip => /> &1 &2 ? H*. 
+      split; [rewrite -H #smt:(@NBytes) |] => ? resultL resultR H0 k??. 
+      rewrite initE ifT 1:/# => />.
+      by rewrite ifT //= H0 get_to_list.
 seq 2 2 : (#pre).
     + inline {1} M(Syscall).__set_key_and_mask; ecall {1} (addr_to_bytes_correctness addr{1}); auto => /> /#.
 seq 2 1 : (
   #pre /\ 
-  (forall (k : int), 0 <= k < 32 => bitmask{1}.[32 + k] = nth witness bitmask_1{2} k) /\
-  size bitmask_1{2} = n
+  (forall (k : int), 0 <= k < 32 => bitmask{1}.[32 + k] = nth witness (val bitmask_1{2}) k)
 ). 
     + inline {1} M(Syscall).__prf_ M(Syscall)._prf; wp; sp.
-      exists * in_01{1}, key0{1}; elim * => _P1 _P2; call {1} (prf_correctness _P1 _P2); first by split; assumption.
-      skip => /> &1 &2 *.
-      do split; [| | by rewrite size_to_list /#]; move => ???; rewrite initE ifT 1:/#; auto => />; [rewrite ifF /# | rewrite ifT /# ].
- 
+      exists * in_01{1}, key0{1}; elim * => _P1 _P2; call {1} (prf_correctness _P1 _P2); first by smt().
+      skip => /> &1 &2 ?H H0 H1 H2 H3.
+      do split; [rewrite -H #smt:(@NBytes) |] => ??? H4.           
+      split => k??.
+         * rewrite initiE 1:/# => />.  
+           rewrite ifF 1:/#.
+           apply H1 => //.
+         * rewrite initiE 1:/# => />.
+           by rewrite ifT 1:/# H4 get_to_list.
 (* Conseq to simplify #post *) 
 conseq (: _ ==>
   size padding{2} = 32 /\
-  size key{2} = 32 /\
-  size bitmask_0{2} = 32 /\
-  size bitmask_1{2} = 32 /\
-  size _left{2} = 32 /\
-  size _right{2} = 32 /\
   addr{1} = address{2} /\
   (forall (k : int), 0 <= k < 32 => buf{1}.[k] = nth witness padding{2} k) /\
-  (forall (k : int), 0 <= k < 32 => buf{1}.[32 + k] = nth witness key{2} k) /\
-  (forall (k : int), 0 <= k < 64 => buf{1}.[64 + k] = nth witness (nbytexor (_left{2} ++ _right{2}) (bitmask_0{2} ++ bitmask_1{2})) k)
+  (forall (k : int), 0 <= k < 32 => buf{1}.[32 + k] = nth witness (val key{2}) k) /\
+  (forall (k : int), 0 <= k < 64 => buf{1}.[64 + k] = nth witness (bytexor (val _left{2} ++ val _right{2}) (val bitmask_0{2} ++ val bitmask_1{2})) k)
 ).
-    + auto => /> &1 &2 H0 H1 H2 H3 H4 H5 H6 H7 H8 H9 H10 buf_L H11 H12 H13 H14 H15 H16 H17. 
-      apply (eq_from_nth witness). rewrite !size_cat size_to_list H3 H4 /nbytexor !size_map !size_zip !size_cat H1 H2 H6 H10 !nval //=.  
-      move => i. rewrite size_to_list => Hi.
+    + auto => /> &1 &2 H0 H1 H2 H3 H4 H5 H6 bufL H7 H8 H9. 
+      apply (eq_from_nth witness). 
+        * rewrite !size_cat H2 /bytexor !size_map size_zip !size_cat.
+          rewrite (: size (val key{2}) = 32) 1:#smt:(NBytes.valP).
+          rewrite (: size (val _left{2}) = 32) 1:#smt:(NBytes.valP).
+          rewrite (: size (val _right{2}) = 32) 1:#smt:(NBytes.valP).
+          rewrite (: size (val bitmask_0{2}) = 32) 1:#smt:(NBytes.valP).
+          rewrite (: size (val bitmask_1{2}) = 32) 1:#smt:(NBytes.valP).
+          rewrite size_iota /#.
+      rewrite size_to_list => i Hi.
       rewrite get_to_list.
-      case (0 <= i < 32). 
-          * smt(@List @Array128).
-      case (32 <= i < 64). 
-          * move => ? _. rewrite nth_cat ifT; first by rewrite size_cat H3 H4 /#. rewrite nth_cat ifF 1:/#. smt(@List @Array128).
+      case (0 <= i < 32); [smt(@List @Array128) |].
+      case (32 <= i < 64).
+        * move => ? _. 
+          rewrite nth_cat.
+          have ->: size (padding{2} ++ val key{2}) = 64 by smt(size_cat NBytes.valP).
+          rewrite ifT 1:/# nth_cat ifF /#. 
       move => Ht0 Ht1. 
       have H: 64 <= i < 128 by smt(). clear Ht0 Ht1 Hi.
-      rewrite nth_cat ifF; first by rewrite size_cat H3 H4 /#.
-      have ->: size (padding{2} ++ key{2}) = 64 by rewrite size_cat H3 H4.
-      smt().
+      rewrite nth_cat.
+      have ->: size (padding{2} ++ val key{2}) = 64 by smt(size_cat NBytes.valP).
+      rewrite ifF /#.
 
-(* End of proof for conseq *)
- 
 while {1} ( 
   0 <= to_uint i{1} <= 64 /\
-
   size padding{2} = 32 /\ 
-  size key{2} = 32 /\
-  size bitmask_0{2} = 32 /\
-  size bitmask_1{2} = 32 /\
-  size _left{2} = 32 /\
-  size _right{2} = 32 /\
-
   addr{1} = address{2} /\
   
-  to_list in_0{1} = _left{2} ++ _right{2} /\
-  to_list bitmask{1} = bitmask_0{2} ++ bitmask_1{2} /\
+  to_list in_0{1} = val _left{2} ++ val _right{2} /\
+  to_list bitmask{1} = val bitmask_0{2} ++ val bitmask_1{2} /\
 
   (forall (k : int), 0 <= k < 32 => buf{1}.[k] = nth witness padding{2} k) /\
-  (forall (k : int), 0 <= k < 32 => buf{1}.[32 + k] = nth witness key{2} k) /\
+  (forall (k : int), 0 <= k < 32 => buf{1}.[32 + k] = nth witness (val key{2}) k) /\
 
   (forall (k : int), 0 <= k < to_uint i{1} => 
     buf{1}.[64 + k] = 
-      nth witness (_left{2} ++ _right{2}) (k) `^` nth witness (bitmask_0{2} ++ bitmask_1{2}) (k))
+      nth witness (val _left{2} ++ val _right{2}) (k) `^` nth witness (val bitmask_0{2} ++ val bitmask_1{2}) (k))
 ) (64 - to_uint i{1}).
-    + auto => /> &hr ?? H0 H1 H2 H3 H4 H5 H6 H7 H8 H9.
-      rewrite /nbytexor => H10 H11; do split; last by smt(@W64 pow2_64).
-       * smt(@W64).
-       * smt(@W64). 
-       * move => *; rewrite get_setE; first by smt(@W64). rewrite ifF; first by smt(@W64 pow2_64). smt(). 
-       * move => *; rewrite get_setE; first by smt(@W64). rewrite ifF; first by smt(@W64 pow2_64). smt(). 
-       * move => k *. 
-         have E0: forall (k : int), 0 <= k < 32 => in_0{hr}.[k] = nth witness _left{m} k by smt(@List @Array64). 
-         have E1: forall (k : int), 0 <= k < 32 => in_0{hr}.[32 + k] = nth witness _right{m} k by smt(@List @Array64). 
-         have E2: forall (k : int), 0 <= k < 32 => bitmask{hr}.[k] = nth witness bitmask_0{m} k by smt(@List @Array64). 
-         have E3: forall (k : int), 0 <= k < 32 => bitmask{hr}.[32 + k] = nth witness bitmask_1{m} k by smt(@List @Array64). 
-         case (0 <= k < 32).
-           - move => ?. rewrite !(nth_cat witness) H2 H4 ifT 1:/# ifT 1:/# get_setE; [smt(@W64) |].
-             case (64 + k = to_uint ((of_int 64)%W64 + i{hr})).
-                + move => ?. congr; have ->: to_uint i{hr} = k by smt(@W64 pow2_64).
-                    - apply E0; smt(). 
-                    - apply E2; smt(). 
-                + move => ?. rewrite H10; first by smt(@W64 pow2_64). congr; rewrite (nth_cat witness) ifT 1:/# //=.
-           - move => H12. rewrite !(nth_cat witness) H2 H4 ifF 1:/# ifF 1:/# get_setE; [smt(@W64) |]. 
-             case (64 + k = to_uint ((of_int 64)%W64 + i{hr})).
-                + move => ?. have ->: to_uint i{hr} = k by smt(@W64 pow2_64). congr; smt(@List @Array64).
-                + move => ?. rewrite H10; first by smt(@W64 pow2_64). 
-                  rewrite !(nth_cat witness) ifF 1:/# ifF 1:/# H2 H4 //. 
-    + auto => /> &1 &2 H0 H1 H2 H3 H4 H5 H6 H7 H8 H9 H10; do split;1..4,6:smt(). 
-       * apply /(eq_from_nth witness); first by rewrite size_cat size_to_list H6 H10 /#.
-         rewrite size_to_list => i?; rewrite nth_cat get_to_list H6; case (i < n); smt(). 
-       * move => bufL iL; do split.
-           - move => *. smt(@W64).
-           - move => Ht0 Ht1 Ht2 H11 H12 H13 H14. 
-             have ->: to_uint iL = 64 by smt(@W64 pow2_64).
-             clear Ht0 Ht1 Ht2.
-             move => H15 H16 H17 H18.
-             move => k Hk0 Hk1. 
-             rewrite /nbytexor (nth_map witness); first by rewrite size_zip !size_cat H1 H2 H6 H10 nval /#. 
-             auto => />.
-             have ->: (nth witness (zip (_left{2} ++ _right{2}) (bitmask_0{2} ++ bitmask_1{2})) k).`1 = nth witness (_left{2} ++ _right{2}) k by smt(@List). 
-             have ->: (nth witness (zip (_left{2} ++ _right{2}) (bitmask_0{2} ++ bitmask_1{2})) k).`2 = nth witness (bitmask_0{2} ++ bitmask_1{2}) k by smt(@List). 
-             apply H18. smt(). 
+    + auto => /> &hr ?? H0 H1 H2 H3 H4 H5 H6.
+      have T: 0 <= to_uint i{hr} < 64 by smt(@W64). 
+      do split;1,2,6:smt(@W64 pow2_64).      
+       * move => k??.   
+         rewrite get_setE 1:#smt:(@W64) ifF 1:#smt:(@W64 pow2_64) /#.       * move => k??.   
+         rewrite get_setE 1:#smt:(@W64) ifF 1:#smt:(@W64 pow2_64) /#.
+       * move => k?. 
+         rewrite to_uintD_small 1:#smt:(@W64) (: to_uint W64.one = 1) 1:/# => ?.  
+         have E0: forall (k : int), 0 <= k < 32 => in_0{hr}.[k] = nth witness (val _left{m}) k by smt(@List @Array64 @NBytes). 
+         have E1: forall (k : int), 0 <= k < 32 => in_0{hr}.[32 + k] = nth witness (val _right{m}) k by smt(@List @Array64 @NBytes). 
+         have E2: forall (k : int), 0 <= k < 32 => bitmask{hr}.[k] = nth witness (val bitmask_0{m}) k by smt(@List @Array64 @NBytes). 
+         have E3: forall (k : int), 0 <= k < 32 => bitmask{hr}.[32 + k] = nth witness (val bitmask_1{m}) k by smt(@List @Array64 @NBytes).
+         rewrite get_setE 1:#smt:(@W64).
+         rewrite to_uintD_small 1:#smt:(@W64) of_uintK //=. 
+         case (64 + k = 64 + to_uint i{hr}) => *; last by apply H5; smt(@W64 pow2_64).
+         rewrite nth_cat (: size (val _left{m}) = 32) 1:#smt:(NBytes.valP).  
+         have ->: to_uint i{hr} = k by smt(@W64 pow2_64).
+         congr; [smt(@List @Array64) |].        
+         rewrite nth_cat (: size (val bitmask_0{m}) = 32) 1:#smt:(NBytes.valP) /#.
+
+    + auto => /> &1 &2 H0 H1 H2 H3 H4 H5 H6; do split; 2:smt().
+        * apply (eq_from_nth witness). 
+             - by rewrite size_to_list size_cat (: size (val bitmask_0{2}) = 32) 1:#smt:(NBytes.valP) (: size (val bitmask_1{2}) = 32) 1:#smt:(NBytes.valP).
+          rewrite size_to_list => j?.
+          rewrite get_to_list. 
+          case (0 <= j < 32) => ?.        
+             - rewrite nth_cat (: size (val bitmask_0{2}) = 32) 1:#smt:(NBytes.valP).   
+               rewrite ifT /#.
+             - rewrite nth_cat (: size (val bitmask_0{2}) = 32) 1:#smt:(NBytes.valP).   
+               rewrite ifF /#.
+        * move => bufL iL; do split.
+             - move => *; smt(@W64).
+             - move => Ht0 Ht1 Ht2 H11 H12 H13 H14. 
+               move => k Hk0 Hk1. 
+               rewrite /bytexor (nth_map witness). 
+                  + rewrite size_zip !size_cat.            
+                    have ->: size (val _left{2}) = 32 by smt(NBytes.valP).
+                    have ->: size (val _right{2}) = 32 by smt(NBytes.valP).
+                    have ->: size (val bitmask_0{2}) = 32 by smt(NBytes.valP).
+                    have ->: size (val bitmask_1{2}) = 32 by smt(NBytes.valP).
+                    smt(). 
+               auto => />.
+               have ->: (nth witness (zip (val _left{2} ++ val _right{2}) (val bitmask_0{2} ++ val bitmask_1{2})) k).`1 = nth witness (val _left{2} ++ val _right{2}) k by smt(@List @NBytes). 
+               have ->: (nth witness (zip (val _left{2} ++ val _right{2}) (val bitmask_0{2} ++ val bitmask_1{2})) k).`2 = nth witness (val bitmask_0{2} ++ val bitmask_1{2}) k by smt(@List @NBytes). 
+               apply H14.
+               smt(@W64 pow2_64).
 qed.
