proof/correctness/Correctness_Address.ec
@@ -4,9 +4,9 @@ require import AllCore List Distr RealExp IntDiv.
 
 from Jasmin require import JModel.
 
-require import Array8.
+require import Array8 Array32.
 
-require import Types Address.
+require import Address.
 require import XMSS_IMPL.
 
 op zero_addr : adrs = Array8.init (fun _ => W32.zero). 
@@ -15,13 +15,43 @@ lemma zero_addr_op_impl (address : adrs) :
     hoare[M(Syscall)._zero_address : true ==> res = zero_addr].
 proof.
 proc.
-while (0 <= i <= 8 /\ 
-      (forall (k : int), 0 <= k < i => (addr.[k] = W32.zero))); auto => /> ; smt(get_setE tP initiE).
+while (
+  0 <= i <= 8 /\ 
+  (forall (k : int), 0 <= k < i => (addr.[k] = W32.zero))
+).
+    + auto => /> &hr *; do split;1,2:smt().
+      move => k??. 
+      rewrite get_setE //= /#.
+    + auto => /> &hr *; split => [/# |].
+      move => addr0 i0 ???. 
+      have ->: i0 = 8 by smt(). 
+      move => H.
+      rewrite /zero_addr tP => j?. 
+      rewrite initiE //=.
+      apply H => //.
 qed.
 
-(* TODO: Move this to termination.ec *)
 lemma zero_addr_ll : islossless M(Syscall)._zero_address by proc; while (true) (8 - i); auto => /> /#.
 
 lemma zero_addr_res (address : adrs) :
     phoare[M(Syscall)._zero_address : true ==> res = zero_addr] = 1%r
       by conseq zero_addr_ll (zero_addr_op_impl address) => //=. 
+
+lemma _addr_to_bytes_correctness (x : W32.t Array8.t) : 
+    hoare[M(Syscall).__addr_to_bytes : 
+        arg.`2 = x ==> to_list res = addr_to_bytes x].
+proof.
+proc.
+admit. 
+qed.
+
+lemma addr_to_bytes_ll : islossless M(Syscall).__addr_to_bytes by proc; inline; while (true) (8 - i); auto => /> /#.
+
+lemma addr_to_bytes_correctness (x : W32.t Array8.t) : 
+    phoare[M(Syscall).__addr_to_bytes : arg.`2 = x ==> 
+      to_list res = addr_to_bytes x] = 1%r.
+proof.
+proc.
+(* conseq addr_to_bytes_ll (_addr_to_bytes_correctness x). *)
+admit.
+qed.
