proof/correctness/Correctness_Conditions.ec
@@ -10,21 +10,21 @@ lemma test_8_bool (b1 b2 : bool) :
   (! (TEST_8 (SETcc b1) (SETcc b2)).`5) = ( b1 /\ b2 ).
 proof.
 rewrite /SETcc /TEST_8.
-case b1; last by smt().
-case b2; [ move => ? ? => //=; smt(@W8) | move => ? => //= ].
+case b1 => [| /#].
+case b2; move => ? ? => //=; smt(@W8). 
 qed.
 
 lemma cmp_W64 :
     forall (a b : W64.t), (! (CMP_64 a b).`2) = (b \ule a).
 move => a b.
-case (b \ule a); by move => ? ; rewrite /CMP_64 /rflags_of_aluop //=; smt(@W64).
+case (b \ule a); by move => ? ; rewrite /CMP_64 /rflags_of_aluop //= #smt:(@W64).
 qed.
 
 lemma cmp_eq_W32 :
     forall (a b : W32.t), (CMP_32 a b).`5 = (a = b).
 proof.
 move => a b.
-case (a = b); move => ?; rewrite /CMP_32 /rflags_of_aluop //=; smt(@W32).
+case (a = b); move => ?; rewrite /CMP_32 /rflags_of_aluop //= #smt:(@W32).
 qed.
 
 lemma test_cmp_32_64 (_a _b : W64.t) (_c _d : W32.t) :
@@ -43,6 +43,6 @@ lemma cond_u64_geq_u64_u32_eq_u32(_a : W64.t, _b : W64.t, _c : W32.t, _d :W32.t)
 proof.
 proc.
 auto => />.
-rewrite /_uGE /_EQ /_uLT /_NEQ /_EQ.
-smt(test_cmp_32_64).
+rewrite /_uGE /_EQ /_uLT /_NEQ /_EQ #smt:(test_cmp_32_64).
 qed.
+
