proof/correctness/Utils2.ec
@@ -1,0 +1,19 @@
+pragma Goals : printall.
+
+require import AllCore List RealExp IntDiv.
+require import BitEncoding.
+(*---*) import BitChunking.
+
+from Jasmin require import JModel.
+
+(** -------------------------------------------------------------------------------------------- **)
+
+pred valid_ptr (p o : W64.t) = 
+  0 <= to_uint o => 
+    0 <= to_uint p /\ to_uint (p + o) < W64.modulus.
+
+pred valid_ptr_i (p : W64.t) (o : int) = 
+  0 <= o => 
+    0 <= to_uint p /\ to_uint (p) + o < W64.modulus.
+
+(** -------------------------------------------------------------------------------------------- **)
